src/Atomic.v
@@ -1,0 +1,205 @@
+Require Import Bool List String Peano_dec.
+Require Import Common ListSupport FMap Syntax Semantics StepDet Serial.
+Require Import Synthesis TrsInv TrsSim.
+
+(* Want:
+ * 1) [AtomicRules] -> [Atomic] -> [steps_det] -> [CompAtomic].
+ * 2) [CompAtomic] is compositional.
+ *)
+
+Section HoareTriple.
+
+  Inductive HoareTriple (obj: Object): Precond -> Rule -> Postcond -> Prop :=
+  | HTRule:
+      forall rule postc,
+        In rule (obj_rules obj) ->
+        (rule_postcond rule) ~~> postc ->
+        HoareTriple obj (rule_precond rule) rule postc
+  | HTWeaken:
+      forall prec rule postc,
+        HoareTriple obj prec rule postc ->
+        forall wprec wpostc,
+          wprec --> prec ->
+          postc ==> wpostc ->
+          HoareTriple obj wprec rule wpostc.
+
+  Corollary HTPreWeaken:
+    forall obj prec rule postc,
+      HoareTriple obj prec rule postc ->
+      forall wprec,
+        wprec --> prec ->
+        HoareTriple obj wprec rule postc.
+  Proof.
+    intros.
+    eapply HTWeaken; eauto.
+  Qed.
+
+  Corollary HTPostWeaken:
+    forall obj prec rule postc,
+      HoareTriple obj prec rule postc ->
+      forall wpostc,
+        postc ==> wpostc ->
+        HoareTriple obj prec rule wpostc.
+  Proof.
+    intros.
+    eapply HTWeaken; eauto.
+  Qed.
+
+  Definition GPrecond := TState -> Value -> Prop.
+  Definition GPostcond := TState -> list Msg -> Prop.
+
+  Definition liftPre (oidx: IdxT) (pre: Precond): GPrecond :=
+    fun prest val =>
+      (tst_oss prest)@[oidx] >>=[True] (* [True] or [False]? *)
+      (fun preost => pre preost val).
+
+  Definition liftPost (oidx: IdxT) (post: Postcond): GPostcond :=
+    fun postst outs =>
+      (tst_oss postst)@[oidx] >>=[True]
+      (fun postost => post postost outs).
+
+  
+  
+End HoareTriple.
+
+Section AtomicRules.
+  
+  Variable (tid: IdxT).
+
+  (* Inductive AtomicRules: MsgId -> System -> Prop := *)
+  (* | ARImm: *)
+  (*     forall oidx oinit immr, *)
+  (*       ImmRule oidx immr -> *)
+  (*       AtomicRules (rule_mid immr) *)
+  (*                   [{| obj_idx := oidx; *)
+  (*                       obj_state_init := oinit; *)
+  (*                       obj_rules := immr :: nil |}] *)
+  (* | ARRqRs: *)
+  (*     forall oidx oinit fwds rqr rsb syss, *)
+  (*       RqRsRules tid oidx fwds rqr rsb -> *)
+  (*       Forall (fun systo => AtomicRules (buildMsgId tid oidx (snd systo) rqChn) *)
+  (*                                        (fst systo)) *)
+  (*              (combine syss fwds) -> *)
+  (*       AtomicRules (rule_mid rqr) *)
+  (*                   ({| obj_idx := oidx; *)
+  (*                       obj_state_init := oinit; *)
+  (*                       obj_rules := rqr :: rsb |} *)
+  (*                      :: concat syss). *)
+
+End AtomicRules.
+
+Section CompAtomic.
+  
+  (* Here are necessary requirements of [CompAtomic], moved from [Serial]:
+   * 1) No external output messages are generated until the transaction ends.
+   * 2) When the transaction ends, it outputs a single external message, which
+   *    is the response of the original request.
+   * 3) When the transaction ends, no internal messages about the transaction 
+   *    are left. We ensure it by just tracking the internal messages about
+   *)
+
+  (* Inductive CompAtomic: *)
+  (*   System -> *)
+  (*   Inv (* precondition *) -> *)
+  (*   TInfo -> *)
+  (*   History -> *)
+  (*   MessagePool TMsg -> *)
+  (*   Inv (* postcondition *) -> *)
+  (*   option TMsg -> Prop := *)
+  (* | CAtomicImm: *)
+  (*     forall sys tid rqin rsout prec postc, *)
+  (*       Atomic sys (buildTInfo tid rqin) *)
+  (*              (IlblOuts (Some (toTMsgU rqin)) (rsout :: nil) :: nil) *)
+  (*              (rsout :: nil) -> *)
+  (*       isExternal sys (mid_from (msg_id (tmsg_msg rsout))) = true -> *)
+  (*       CompAtomic sys prec (buildTInfo tid rqin) *)
+  (*                  (IlblOuts (Some (toTMsgU rqin)) (rsout :: nil) :: nil) *)
+  (*                  nil postc (Some rsout) *)
+
+End CompAtomic.
+
+Section Compositionality.
+
+  Variables
+    (rqin: MsgId)
+    (rqfwds: list MsgId)
+    (rsbacks: list MsgId)
+    (rsout: MsgId)
+
+    (rqfwdR: Rule)
+    (rssbRs: list Rule)
+    (subRs: list Rule)
+    
+    (sim: TState -> TState -> Prop)
+    (p: Label -> Label)
+
+    (spec: System).
+
+  (* FIXME: remove [sys] and [ssys], and replace all uses with appropriate systems. *)
+  Variables (sys ssys: System).
+
+  Local Infix "≈" := sim (at level 30).
+
+  Local Definition rqfwdTMsgs (v: Value) (ti: TInfo) :=
+    map (fun mid => toTMsg ti {| msg_id := mid; msg_value := v |}) rqfwds.
+
+  Definition SimRqF :=
+    forall ist1 sst1,
+      ist1 ≈ sst1 ->
+      forall ist2 v ti,
+        step_det sys ist1 (IlblOuts (Some (toTMsgU (buildMsg rqin v)))
+                                    (rqfwdTMsgs v ti)) ist2 ->
+        ist2 ≈ sst1.
+
+  Definition SimRs :=
+    forall ist1 sst1,
+      ist1 ≈ sst1 ->
+      forall ti rsb rsv ist2,
+        In rsb rsbacks ->
+        step_det sys ist1 (IlblOuts (Some (toTMsg ti (buildMsg rsb rsv))) nil) ist2 ->
+        ist2 ≈ ist1.
+
+  Definition SimRsB :=
+    forall ist1 sst1,
+      ist1 ≈ sst1 ->
+      forall ti rsb rsv ist2,
+        In rsb rsbacks ->
+        step_det sys ist1 (IlblOuts (Some (toTMsg ti (buildMsg rsb rsv)))
+                                    (toTMsg ti (buildMsg rsb rsv) :: nil)) ist2 ->
+        exists slbl sst2,
+          step_det spec sst1 slbl sst2 /\
+          extLabel spec (getLabel slbl) =
+          Some (p (LblOuts (buildMsg rsb rsv :: nil))) /\
+          ist2 ≈ sst2.
+
+  Definition SubAtomicSim :=
+    forall ti hst mouts,
+      Atomic ssys ti hst mouts ->
+      forall ist1 sst1,
+        ist1 ≈ sst1 ->
+        forall ist2,
+          steps_det ssys ist1 hst ist2 ->
+          exists (sst2 : TState) (shst : list TLabel),
+            steps_det spec sst1 shst sst2 /\
+            map p (behaviorOf ssys hst) = behaviorOf spec shst /\
+            ist2 ≈ sst2.
+
+  Hypotheses (Hrqf: SimRqF) (Hrs: SimRs) (Hrsb: SimRsB)
+             (Hsub: SubAtomicSim).
+
+  Theorem atomic_sim_compositional:
+    forall ti hst mouts,
+      Atomic sys ti hst mouts ->
+      forall ist1 sst1,
+        ist1 ≈ sst1 ->
+        forall ist2,
+          steps_det ssys ist1 hst ist2 ->
+          exists (sst2 : TState) (shst : list TLabel),
+            steps_det spec sst1 shst sst2 /\
+            map p (behaviorOf ssys hst) = behaviorOf spec shst /\
+            ist2 ≈ sst2.
+  Proof.
+  Admitted.
+
+End Compositionality.
+
